working on a new (hopefully more principled) version of expression unification.

src/ExprUnify2.v
@@ -1,24 +1,97 @@
 Require Import Expr.
 Require Import NatMap.
 Require Import EquivDec.
-Require Import List.
+Require Import List Bool.
+
+Set Implicit Arguments.
+Set Strict Implicit.
 
 Module SUBST := NatMap.IntMap.
 
 Section typed.
   Variable types : list type.
 
-  Definition Subst :=
-    @SUBST.t (expr types).
+  Check fold_right.
+
+  Fixpoint uvars_of (e : expr types) : list nat :=
+    match e with
+      | Const _ _ 
+      | Var _ => nil
+      | UVar n => n :: nil
+      | Func _ args => fold_right (fun x a => a ++ uvars_of x) nil args
+      | Equal _ l r => uvars_of l ++ uvars_of r
+    end.
+  
+  Definition Subst : Type :=
+    SUBST.t (expr types).
+
+  Definition Subst_lookup (k : nat) (s : Subst) : option (expr types) :=
+    SUBST.find k s.
+
+  Section Instantiate.
+    Variable sub : Subst.
+
+    Fixpoint exprInstantiate (e : expr types) : expr types :=
+      match e with 
+        | Const _ _ 
+        | Var _ => e
+        | UVar n => match Subst_lookup n sub with
+                      | None => e 
+                      | Some v => v
+                    end
+        | Func f args => Func f (map exprInstantiate args)
+        | Equal t l r => Equal t (exprInstantiate l) (exprInstantiate r)
+      end.
+  End Instantiate.
+
+  Section SubstDenote.
+    Variable funcs : functions types.
+    Variable vars : env types.
+    Variable sub : Subst.
+
+    Fixpoint Subst_equations (ls : env types) (cur : nat) : env types -> Prop :=
+      match ls with
+        | nil => fun _ => True
+        | l :: ls =>
+          let P := Subst_equations ls (S cur) in
+          match Subst_lookup cur sub with
+            | None => P
+            | Some v => fun g => 
+              match exprD funcs g vars v (projT1 l) with 
+                | Some v => v = projT2 l
+                | None => False
+              end /\ P g
+          end
+      end.
+  End SubstDenote.
 
   Definition empty_Subst : Subst :=
     SUBST.empty.
 
-  Definition Subst_lookup (k : nat) (s : Subst) :=
-    SUBST.find k s.
+  Fixpoint allb T (F : T -> bool) (ls : list T) : bool :=
+    match ls with
+      | nil => true
+      | l :: ls => F l && allb F ls
+    end.
 
-  Definition Subst_replace (k : nat) (v : expr types) (s : Subst) :=
-    SUBST.add k v s.
+  Definition consistentb (k : nat) (e : expr types) : bool :=
+    if In_dec equiv_dec k (uvars_of e) then false else true.
+
+  Definition Subst_replace (k : nat) (v : expr types) (s : Subst) : option Subst :=
+    let v' := exprInstantiate s v in
+    if In_dec equiv_dec k (uvars_of v') then
+      None
+    else
+      let s := SUBST.add k v' s in
+      let s := SUBST.map (fun _ => exprInstantiate s) s in
+      SUBST.fold (fun k e acc => match acc with
+                                   | None => None
+                                   | Some acc => 
+                                     let e := exprInstantiate s e in
+                                     if consistentb k e then
+                                       Some (SUBST.add k e acc)
+                                     else None
+                                 end) s (Some s).
 
   Definition get_Eq (t : tvar) : forall x y : tvarD types t, option (x = y) :=
     match t as t return forall x y : tvarD types t, option (x = y) with
@@ -38,6 +111,10 @@ Section typed.
         end 
     end.
 
+  (** index by a bound, since the termination argument is not trivial
+   ** it is guaranteed to not make more recursions than the number of
+   ** uvars.
+   **)
   Fixpoint exprUnify (l r : expr types) (sub : Subst) : option Subst.
   refine (
     match l , r with
@@ -95,57 +172,76 @@ Section typed.
     end).
   Defined.
 
-  Check Expr.forallEach.
-
-
-
-  Variable funcs : functions types.
-
-  Fixpoint Subst_existsEach (ls : variables) (sub : Subst) (cur : nat)
-    (P : env types -> (env types -> Prop) -> Prop) : Prop :=
-    match ls with
-      | nil => P nil (fun _ => True)
-      | l :: ls =>
-        exists x : tvarD types l, 
-          Subst_existsEach ls sub (S cur) (fun g p => 
-            let env' := @existT _ (tvarD types) _ x :: g in
-            match Subst_lookup cur sub with
-              | None => P env' p
-              | Some v => P env' (fun env => 
-                exprD funcs env nil v l = Some x /\ p env)
-            end)
-    end.
-
-  Theorem exprUnify_correct : forall env uvars l r t sub sub',
-    exprUnify l r sub = Some sub' ->
-    Subst_existsEach uvars sub' 0 (fun uenv eqs => 
+  (** Syntactic Unification **)
+  Section Unifies.
+    Variable funcs : functions types.
+    Variable vars : env types.
+    
+    (** NOTE: the meaning of Prop isn't quite perfect. We currently reflect Props
+     ** but we actually mean proofs, i.e. using the Provable predicate.
+     **)
+    Definition unifies uenv env (t : tvar) (l r : expr types) : Prop :=
       match exprD funcs uenv env l t , exprD funcs uenv env r t with
-        | Some l , Some r => l = r
+        | Some l , Some r => match t as t return tvarD types t -> tvarD types t -> Prop with
+                               | tvProp => fun l r => l <-> r (** we'll weaken things a bit more **)
+                               | tvType _ => fun l r => l = r
+                             end l r
         | _ , _ => False
-      end /\ eqs uenv) ->
-    Subst_existsEach uvars sub 0 (fun uenv eqs => 
-      match exprD funcs uenv env l t , exprD funcs uenv env r t with
-        | Some l , Some r => l = r
-        | _ , _ => False
-      end /\ eqs uenv).
-  Proof.
-    induction l; destruct r; simpl; intros; try congruence.
-    Focus. (** Const **)
-      destruct (equiv_dec t t1); try congruence.
-      generalize dependent t2.
-      generalize e. rewrite <- e. admit. (** this case is problematic **)
+      end.
+  End Unifies.
 
-    Focus. (** Var **)
-    destruct (Peano_dec.eq_nat_dec x x0); try congruence.
-    inversion H; clear H; subst; eauto.
 
-    Focus. (** Equal **)
-    destruct (equiv_dec t t0); try congruence.
-    revert H2; case_eq (exprUnify l1 r1 sub); intros; try congruence.
-    eapply IHl1 with (t := t) in H.
-    eapply IHl2 with (t := t) in H2.
-  Admitted.
+  Section Correctness.
+    Variable funcs : functions types.
+    Variable vars : env types.
 
+    Theorem exprUnify_correct : forall env uvars l r t sub sub',
+      exprUnify l r sub = Some sub' ->
+      existsEach uvars (fun uenv =>
+        Subst_equations funcs env sub uenv 0 uenv /\  
+        is_well_typed funcs uenv env l t = true /\ 
+        is_well_typed funcs uenv env r t = true) ->
+      existsEach uvars (fun uenv =>
+        Subst_equations funcs env sub' uenv 0 uenv /\  
+        unifies funcs uenv env t l r).
+    Proof.
+      induction l; destruct r; intuition; simpl in *; try congruence;
+        repeat (match goal with 
+                  | [ H : existsEach _ _ |- _ ] => 
+                    apply existsEach_sem in H
+                  | [ H : exists x, _ |- _ ] => destruct H
+                  | [ H : match ?X with 
+                            | left _ => _
+                            | right _ => _ 
+                          end = _ |- _ ] => destruct X; try congruence
+                  | [ H : Some _ = Some _ |- _ ] => inversion H; clear H; subst
+                  | [ H : match ?X with 
+                            | None => _
+                            | Some _ => _ 
+                          end = _ |- _ ] => revert H; case_eq X; intros; try congruence
+                end; intuition; unfold equiv in *; subst); 
+        eapply existsEach_sem.
+      Focus. (** const **)
+        exists x; intuition. unfold unifies; simpl. repeat rewrite EquivDec_refl_left.
+        destruct t3; intuition auto.
+      
+      Focus. (** var **)
+        exists x1; intuition eauto.
+        unfold unifies; simpl. rewrite H. destruct t; intuition eauto.
+
+      Focus. (** equal **)
+        destruct t1; try congruence.
+        apply andb_true_iff in H4. apply andb_true_iff in H2.
+        intuition.
+        eapply IHl1 with (t := t0) in H; [ | apply existsEach_sem; exists x; intuition ].
+        apply existsEach_sem in H. destruct H; intuition.
+        eapply IHl2 with (t := t0) in H1; [ | apply existsEach_sem; exists x0; intuition ].
+
+        Focus.
+        apply existsEach_sem in H1. destruct H1; intuition.
+        exists x1; intuition eauto. unfold unifies; simpl.
+    Admitted.
+  End Correctness.
 
 End typed.
 
@@ -156,15 +252,19 @@ Module TEST.
   Definition uvars := tvType 0 :: tvType 0 :: tvType 0 :: nil.
   Definition subst := 
     let s := empty_Subst types in
-    Subst_replace types 1 (UVar 0) s.
+    Subst_replace 1 (UVar 0) s.
   Definition funcs : functions types := nil.
 
-  Print Provable.
-
   Goal 
-    Subst_existsEach types funcs uvars subst 0 (fun env other =>
-      Provable funcs env vars_env (Equal (tvType 0) (UVar 0) (UVar 2)) /\ other env).
+    existsEach uvars (fun uenv =>
+      match subst with 
+        | None => False
+        | Some subst => 
+          Subst_equations funcs vars_env subst uenv 0 uenv 
+      end /\  
+      AllProvable funcs uenv vars_env 
+        ((Equal (tvType 0) (UVar 0) (UVar 2)) :: 
+         (Equal (tvType 0) (UVar 0) (@Const types (tvType 0) 3)) :: nil)).
     compute.
-    do 3 eexists.
   Abort.
 End TEST.
